FypSchedulingAlgorithms/Process.lean
@@ -8,6 +8,7 @@ structure AperiodicProcess where
   arrival   : Nat
   burst     : Nat
   remaining : Nat
+  burst_exceed_zero : burst > 0
 deriving BEq, Repr
 
 -- #eval AperiodicProcess.mk 1 0 5 5
@@ -19,13 +20,14 @@ structure PeriodicProcess where
   burst     : Nat
   deadline  : Nat
   remaining : Nat
+  burst_exceed_zero : burst > 0
   -- Add `valid` back in if turns out the inequalities are useful in the proof
-  -- valid     : remaining ≤ burst ∧ burst ≤ deadline ∧ deadline ≤ period
+  -- valid     : 0 < burst ∧ remaining ≤ burst ∧ burst ≤ deadline ∧ deadline ≤ period
 deriving BEq, Repr
 
--- #eval PeriodicProcess.mk 1 0 10 5 7 5 ⟨by omega, by omega, by omega⟩
+-- #eval PeriodicProcess.mk 1 0 10 5 7 5 (by omega) ⟨by omega, by omega, by omega, by omega⟩
 
-#eval PeriodicProcess.mk 1 0 10 5 7 5
+#eval PeriodicProcess.mk 1 0 10 5 7 5 (by omega)
 
 class Process (α : Type) extends BEq α where
   id            : α → Nat
@@ -38,6 +40,8 @@ class Process (α : Type) extends BEq α where
   -- Let arrival stream be a function that takes time as argument and returns list of arriving processes
   convert_to_arrival_stream : List α → Nat → List α
   tick_decrements : ∀ p, remaining (tick p) = remaining p - 1
+  id_invariant_wrt_tick : ∀ p, id (tick p) = id (p)
+  burst_exceed_zero : ∀ p, burst (p) > 0
 
 instance : Process AperiodicProcess where
   id p := p.id
@@ -51,6 +55,8 @@ instance : Process AperiodicProcess where
     fun current_time =>
       original_process_list.filter (fun p => current_time = p.arrival)
   tick_decrements _p := rfl
+  id_invariant_wrt_tick _p := rfl
+  burst_exceed_zero p := p.burst_exceed_zero
 
 instance : Process PeriodicProcess where
   id p := p.id
@@ -64,3 +70,5 @@ instance : Process PeriodicProcess where
     fun current_time =>
       original_process_list.filter (fun p => current_time % p.arrival = 0)
   tick_decrements _p := rfl
+  id_invariant_wrt_tick _p := rfl
+  burst_exceed_zero p := p.burst_exceed_zero
